Mica/SourceTinyML.lean
@@ -4,6 +4,8 @@ import Mica.SourceTinyML.Types
 import Mica.SourceTinyML.Untyped
 import Mica.SourceTinyML.Typed
 import Mica.SourceTinyML.Spec
+import Mica.SourceTinyML.Assertions
+import Mica.SourceTinyML.TypeConstraints
 import Mica.SourceTinyML.Typing
 import Mica.SourceTinyML.Printer
 import Mica.SourceTinyML.World
